lab_to_targetProof: compile_correct done

compiler/backend/proofs/lab_to_targetProofScript.sml
@@ -664,7 +664,7 @@ Definition share_mem_domain_code_rel_def:
           i <= index /\
           find_index (p + n2w (pos_val pc 0 code2)) mc_conf.ffi_entry_pcs 0 =
             SOME index /\
-          (let (name, nb) = get_memop_info op (:'a) in
+          (let (name, nb) = get_memop_info op in
             EL index mc_conf.ffi_names = name /\
             mc_conf.mmio_info index =
               (nb, a, re, p + n2w (pos_val pc 0 code2 + len))))) /\
@@ -697,12 +697,13 @@ Definition share_mem_state_rel_def:
         (t1 with pc := EL index mc_conf.ffi_entry_pcs) ms2 ==>
         (* If we are doing mapped read, and addresses are fine *)
         (EL index mc_conf.ffi_names = "MappedRead" /\
-        (w2n ad' MOD w2n nb) = 0 /\ (ad' IN mc_conf.shared_addresses) /\
+         (if nb = 0w then (w2n ad' MOD (dimindex (:'a) DIV 8)) = 0
+          else T) /\ (ad' IN mc_conf.shared_addresses) /\
          is_valid_mapped_read (mc_conf.target.get_pc ms2) nb (Addr ad offs) re pc'
            mc_conf.target ms2 mc_conf.prog_addresses /\
          call_FFI st "MappedRead"
            [nb]
-           (addr2w8list ad') =
+           (word_to_bytes ad' F) =
            FFI_return new_st new_bytes ==>
           target_state_rel mc_conf.target
             (t1 with
@@ -712,13 +713,16 @@ Definition share_mem_state_rel_def:
               (mc_conf.ffi_interfer k (index,new_bytes,ms2))) /\
         (* If we are doing mapped write, and the addresses are fine *)
         (EL index mc_conf.ffi_names = "MappedWrite" /\
-         (w2n ad' MOD w2n nb) = 0 /\ (ad' IN mc_conf.shared_addresses) /\
+         (if nb = 0w then (w2n ad' MOD (dimindex (:'a) DIV 8)) = 0
+          else T) /\ (ad' IN mc_conf.shared_addresses) /\
           is_valid_mapped_write (mc_conf.target.get_pc ms2) nb (Addr ad offs) re pc'
             mc_conf.target ms2 mc_conf.prog_addresses /\
          call_FFI st "MappedWrite"
           [nb]
-          (w2wlist_le (mc_conf.target.get_reg ms2 re) (w2n nb)
-                    ++ (addr2w8list ad')) =
+          ((let w = mc_conf.target.get_reg ms2 re in
+              if nb = 0w then word_to_bytes w F
+              else word_to_bytes_aux (w2n nb) w F)
+           ++ (word_to_bytes ad' F)) =
           FFI_return new_st new_bytes ==>
           target_state_rel mc_conf.target
             (t1 with pc := pc')
@@ -1844,6 +1848,8 @@ val share_mem_state_rel_tac =
   gvs[IMP_CONJ_THM, AND_IMP_INTRO]
   >- (first_x_assum $ ho_match_mp_tac o cj 1 >> fs[] >> metis_tac[])
   >- (first_x_assum $ ho_match_mp_tac o cj 2 >> fs[] >> metis_tac[])
+  >- (first_x_assum $ ho_match_mp_tac o cj 1 >> fs[] >> metis_tac[])
+  >- (first_x_assum $ ho_match_mp_tac o cj 2 >> fs[] >> metis_tac[])
 
 Theorem Inst_lemma:
   ~(asm_inst i s1).failed /\
@@ -1913,6 +1919,8 @@ Proof
     conj_tac >- (
     fs[upd_pc_def, inc_pc_def, arith_upd_def, share_mem_state_rel_def] >> rw[]>>
     gvs[IMP_CONJ_THM, AND_IMP_INTRO]
+    >- (first_x_assum $ ho_match_mp_tac o cj 1 >> fs[] >> metis_tac[])
+    >- (first_x_assum $ ho_match_mp_tac o cj 2 >> fs[] >> metis_tac[])
     >- (first_x_assum $ ho_match_mp_tac o cj 1 >> fs[] >> metis_tac[])
     >- (first_x_assum $ ho_match_mp_tac o cj 2 >> fs[] >> metis_tac[])) >>
     fs[upd_pc_def,inc_pc_def,arith_upd_share_mem_domain_unchange])
@@ -6196,199 +6204,16 @@ fun map_first_cj t =
   MAP_FIRST ho_match_mp_tac $ gen_list 1
 end
 
-fun reg_val_tac reg =
-  qpat_x_assum `!r. word_loc_val _ _ _ = SOME _` $
-    qspec_then reg assume_tac
-  \\ fs[word_loc_val_def]
-  \\ rfs[word_loc_val_def];
-
 val enc_is_valid_mapped_access_tac =
     fs[is_valid_mapped_read_def,is_valid_mapped_write_def]
-    \\ rfs[enc_with_nop_thm]
-    \\ fs[]
+    \\ fs[enc_with_nop_thm]
+    \\ rfs[]
     \\ drule_then assume_tac $
         cj 1 $ cj 1 $ PURE_REWRITE_RULE [EQ_IMP_THM] bytes_in_memory_APPEND
     \\ drule_then assume_tac bytes_in_memory_in_domain
     \\ irule bytes_in_memory_change_mem
     \\ qexists `t1.mem`
     \\ simp[];
-
-fun share_mem_load_compile_correct_tac ffi_name new_t1 nb new_ffi =
-  qpat_assum `!i. _ ==> mc_conf.target.get_reg ms1 i = t1.regs i` $
-    qspec_then `n''` drule_all
-  \\ strip_tac
-  \\ fs[call_FFI_def]
-  \\ last_x_assum irule
-  \\ simp[]
-  \\ conj_tac
-  >- (rpt gen_tac
-      \\ strip_tac
-      \\ first_x_assum $ qspecl_then [`ms2`, `t1'`, `k`, `a1`, `a2`] mp_tac
-      \\ simp[] )
-  \\ conj_tac
-  >- (rpt gen_tac
-    \\ simp[apply_oracle_def,shift_interfer_def,shift_seq_def]
-    \\ fs[IMP_CONJ_THM, AND_IMP_INTRO]
-    \\ conj_tac
-    \\ strip_tac
-    \\ first_x_assum map_first_cj
-    \\ fs[]
-    \\ qexistsl [`st`, `new_st`]
-    \\ simp[]
-    \\ irule $ cj 2 RTC_RULES
-    \\ qexists new_ffi
-    \\ simp[evaluatePropsTheory.call_FFI_rel_def]
-    \\ qexists ffi_name
-    \\ simp[call_FFI_def, AllCaseEqs()]
-    \\ metis_tac[] )
-  >- (
-    rpt gen_tac
-    \\ simp[apply_oracle_def,shift_interfer_def,shift_seq_def]
-    \\ conj_tac
-    >- (
-      rpt gen_tac
-      \\ strip_tac
-      \\ first_x_assum $ qspecl_then
-        [`ms2`,`k+1`,`index'`,`new_bytes`,`t1'`,`bytes'`,`bytes2`,`st`,`new_st`]
-        assume_tac
-      \\ first_x_assum ho_match_mp_tac
-      \\ fs[]
-      \\ irule $ cj 2 RTC_RULES
-      \\ qexists new_ffi
-      \\ simp[evaluatePropsTheory.call_FFI_rel_def]
-      \\ qexists ffi_name
-      \\ simp[call_FFI_def, AllCaseEqs()]
-      \\ metis_tac[] )
-    >- (
-      simp[apply_oracle_def,shift_interfer_def,shift_seq_def]
-      \\ first_x_assum $ qspecl_then
-        [`ms1`, `0`,`index`,`v4`, `t1`, nb,`n''`,`c`,`n'`,
-          `p + n2w (LENGTH bytes + pos_val s1.pc 0 code2)`,`s1.ffi`,
-          new_ffi] mp_tac
-      \\ simp[]
-      \\ impl_tac
-      >- (
-        simp[target_state_rel_def]
-        \\ drule find_index_LESS_LENGTH
-        \\ simp[]
-        \\ disch_then kall_tac
-        \\ fs[find_index_INDEX_OF, INDEX_OF_eq_SOME] )
-      \\ impl_tac
-      >- (
-        gvs[is_valid_mapped_write_def,is_valid_mapped_read_def,good_dimindex_def]
-        \\ gvs[enc_with_nop_thm]
-        \\ drule $ cj 1 $ cj 1 $ PURE_REWRITE_RULE [EQ_IMP_THM] bytes_in_memory_APPEND
-        \\ strip_tac
-        \\ drule_all bytes_in_memory_eq_mem
-        \\ simp[]
-      )
-      \\ strip_tac
-      \\ fs[target_state_rel_def]
-      \\ qexistsl [`code2`, new_t1]
-      \\ rw[]
-      >- (first_x_assum irule >> metis_tac[])
-      \\ simp[APPLY_UPDATE_THM]
-      \\ IF_CASES_TAC
-      \\ fs[word_loc_val_def]
-    )
-  );
-
-fun share_mem_store_compile_correct_tac ffi_name new_t1 (nb: term frag list) new_ffi =
-  let
-    val (wnb: term frag list) = `n2w (` @ nb @ `)`
-  in
-  qpat_assum `!i. _ ==> mc_conf.target.get_reg ms1 i = t1.regs i` $
-    qspec_then `n''` drule_all
-  \\ rpt strip_tac
-  \\ `mc_conf.target.get_reg ms1 n' = t1.regs n'` by (
-        qpat_x_assum `!i. _ ==> mc_conf.target.get_reg ms1 i = t1.regs i` $
-          qspec_then `n'` irule
-        \\ simp[] )
-  \\ `(dimindex (:α) DIV 8) MOD 256 = dimindex (:α) DIV 8` by fs[good_dimindex_def]
-  \\ gvs[call_FFI_def,LENGTH_APPEND,inc_pc_def,dec_clock_def]
-  \\ last_x_assum irule
-  \\ simp[]
-  \\ conj_tac
-  >- (rpt gen_tac
-      \\ strip_tac
-      \\ first_x_assum $ qspecl_then [`ms2`, `t1'`, `k`, `a1`, `a2`] mp_tac
-      \\ simp[] )
-  \\ conj_tac
-  >- (rpt gen_tac
-    \\ simp[apply_oracle_def,shift_interfer_def,shift_seq_def]
-    \\ fs[IMP_CONJ_THM, AND_IMP_INTRO]
-    \\ conj_tac
-    \\ strip_tac
-    \\ first_x_assum map_first_cj
-    \\ fs[]
-    \\ qexistsl [`st`, `new_st`]
-    \\ simp[]
-    \\ irule $ cj 2 RTC_RULES
-    \\ qexists new_ffi
-    \\ simp[evaluatePropsTheory.call_FFI_rel_def]
-    \\ qexists ffi_name
-    \\ simp[call_FFI_def, AllCaseEqs()]
-    \\ qexistsl [
-      `[` @ wnb @ `]`,
-      `w2wlist_le (t1.regs n') (`  @ nb @ `) ++ addr2w8list (c + t1.regs n'')`,
-      `v4`, `ffi'`]
-    \\ gvs[LENGTH_APPEND] )
-  >- (
-    rpt gen_tac
-    \\ simp[apply_oracle_def,shift_interfer_def,shift_seq_def]
-    \\ conj_tac
-    >- (
-      rpt gen_tac
-      \\ strip_tac
-      \\ first_x_assum $ qspecl_then
-        [`ms2`,`k+1`,`index'`,`new_bytes`,`t1'`,`bytes'`,`bytes2`,`st`,`new_st`]
-        assume_tac
-      \\ first_x_assum ho_match_mp_tac
-      \\ fs[]
-      \\ irule $ cj 2 RTC_RULES
-      \\ qexists new_ffi
-      \\ simp[evaluatePropsTheory.call_FFI_rel_def]
-      \\ qexists ffi_name
-      \\ simp[call_FFI_def, AllCaseEqs()]
-      \\ qexistsl [
-        `[` @ wnb @ `]`,
-        `w2wlist_le (t1.regs n') (`  @ nb @ `) ++ addr2w8list (c + t1.regs n'')`,
-        `v4`, `ffi'`]
-      \\ fs[LENGTH_APPEND] )
-    >- (
-      simp[apply_oracle_def,shift_interfer_def,shift_seq_def]
-      \\ first_x_assum $ qspecl_then
-        [`ms1`, `0`,`index`,`v4`, `t1`, wnb,`n''`,`c`,`n'`,
-          `p + n2w (LENGTH bytes + pos_val s1.pc 0 code2)`,`s1.ffi`,
-          new_ffi] mp_tac
-      \\ simp[]
-      \\ impl_tac
-      >- (
-        simp[target_state_rel_def]
-        \\ drule find_index_LESS_LENGTH
-        \\ simp[]
-        \\ disch_then kall_tac
-        \\ fs[find_index_INDEX_OF, INDEX_OF_eq_SOME] )
-      \\ impl_tac
-      >- (
-        gvs[is_valid_mapped_write_def,is_valid_mapped_read_def,good_dimindex_def]
-        \\ gvs[enc_with_nop_thm]
-        \\ drule $ cj 1 $ cj 1 $ PURE_REWRITE_RULE [EQ_IMP_THM] bytes_in_memory_APPEND
-        \\ strip_tac
-        \\ drule_all bytes_in_memory_eq_mem
-        \\ simp[]
-      )
-      \\ strip_tac
-      \\ fs[target_state_rel_def]
-      \\ qexistsl [`code2`, new_t1]
-      \\ rw[]
-      >- (first_x_assum irule >> metis_tac[])
-      \\ simp[APPLY_UPDATE_THM]
-      \\ IF_CASES_TAC
-      \\ fs[word_loc_val_def]
-    )
-  )
-end
 
 Theorem ffi_entry_pcs_NOT_ccache_OR_halt_pc:
    find_index pc mc_conf.ffi_entry_pcs 0 =
@@ -6401,36 +6226,6 @@ Proof
   rpt strip_tac >>
   gvs[find_index_INDEX_OF,INDEX_OF_eq_SOME]
 QED
-
-val share_mem_eval_expand_tac =
-  fs[share_mem_op_def,share_mem_load_def,share_mem_store_def,AllCaseEqs(),call_FFI_def]
-  \\ simp[Once targetSemTheory.evaluate_def]
-  \\ fs[state_rel_def,share_mem_domain_code_rel_def,asm_fetch_def,
-    ELIM_UNCURRY,get_memop_info_def]
-  \\ drule_all $ GEN_ALL IMP_bytes_in_memory_ShareMem
-  \\ strip_tac
-  \\ qpat_assum `!pc op re a inst len i. asm_fetch_aux _ _ = SOME _ /\
-      mmio_pcs_min_index _ = SOME _ ==> _` drule_all
-  \\ strip_tac
-  \\ drule find_index_is_MEM
-  \\ fs[target_state_rel_def]
-  \\ disch_then kall_tac
-  \\ fs[share_mem_state_rel_def]
-  \\ qpat_assum `!index' i'. mmio_pcs_min_index _ = SOME i' /\ index' < _ /\
-      _ ==> _` $ qspecl_then [`index`, `i`] drule
-  \\ (
-    impl_tac >- (drule find_index_LESS_LENGTH >> fs[])
-    \\ disch_then assume_tac
-    \\ `mc_conf.target.get_pc ms1 <> mc_conf.ccache_pc /\
-        mc_conf.target.get_pc ms1 <> mc_conf.halt_pc` by (
-          irule ffi_entry_pcs_NOT_ccache_OR_halt_pc >> gvs[])
-    \\ rfs[get_memop_info_def]
-    \\ TOP_CASE_TAC
-    \\ fs[labSemTheory.addr_def,AllCaseEqs()]
-    \\ rw[GSYM PULL_EXISTS]
-    \\ `(dimindex (:'a) DIV 8) MOD 256 <> 1` by (rfs[good_dimindex_def] >> fs[])
-    \\ fs[asm_ok_def,inst_ok_def,reg_ok_def]
-  );
 
 Theorem ffi_name_NOT_Mapped:
   mmio_pcs_min_index ffi_names = SOME i /\
@@ -6885,118 +6680,116 @@ Proof
     \\ `^s1.clock - 1 + k + l = ^s1.clock + (k + l - 1)` by decide_tac
     \\ fs[])
   THEN1 (* share_mem_op *)
-  (say "share_mem_op"
-    \\ Cases_on `m`
-    >- ( (* Load *)
-      gvs[pair_case_eq,option_case_eq, ffi_result_case_eq]
-      \\ share_mem_eval_expand_tac
-      \\ `t1.regs n'' = w` by reg_val_tac `n''`
-      \\ simp[]
-      >- (rfs[good_dimindex_def] >> fs[])
-      >- enc_is_valid_mapped_access_tac
-      >- share_mem_load_compile_correct_tac `"MappedRead"`
-          `t1 with
-              <| regs := (n' =+ (word_of_bytes F 0w v4)) t1.regs;
-                pc := p + n2w (LENGTH bytes + pos_val s1.pc 0 code2)|>`
-          `n2w (dimindex (:α) DIV 8)`
-          `s1.ffi with
-            <|ffi_state := ffi';
-              io_events :=
-                s1.ffi.io_events ++
-                [IO_event "MappedRead"
-                  [n2w (dimindex (:α) DIV 8)]
-                  (ZIP (addr2w8list (c + t1.regs n''),v4))]|>`
-      >- (rfs[good_dimindex_def] >> fs[])
-      >- enc_is_valid_mapped_access_tac
-      >- gvs[apply_oracle_def,call_FFI_def]
-      >- (rfs[good_dimindex_def] >> fs[])
-      >- enc_is_valid_mapped_access_tac
-      >- gvs[apply_oracle_def,call_FFI_def]
-    )
-    >- ( (* Load8 *)
-      gvs[pair_case_eq,option_case_eq, ffi_result_case_eq]
-      \\ share_mem_eval_expand_tac
-      \\ `t1.regs n'' = w` by reg_val_tac `n''`
-      \\ simp[]
-      >- enc_is_valid_mapped_access_tac
-      >- share_mem_load_compile_correct_tac `"MappedRead"`
-          `t1 with
-              <| regs := (n' =+ (word_of_bytes F 0w v4)) t1.regs;
-                pc := p + n2w (LENGTH bytes + pos_val s1.pc 0 code2)|>`
-          `1w`
-          `s1.ffi with
-            <|ffi_state := ffi';
-              io_events :=
-                s1.ffi.io_events ++
-                [IO_event "MappedRead"
-                  [1w]
-                  (ZIP (addr2w8list (c + t1.regs n''),v4))]|>`
-      >- enc_is_valid_mapped_access_tac
-      >- gvs[apply_oracle_def,call_FFI_def]
-      >- enc_is_valid_mapped_access_tac
-      >- gvs[apply_oracle_def,call_FFI_def]
-    )
-    >- ( (* Store *)
-      gvs[pair_case_eq,option_case_eq, ffi_result_case_eq]
-      \\ share_mem_eval_expand_tac
-      \\ `t1.regs n'' = w'` by reg_val_tac `n''`
-      \\ simp[]
-      >- (rfs[good_dimindex_def] >> fs[])
-      >- enc_is_valid_mapped_access_tac
-      >- (
-        `t1.regs n' = w` by reg_val_tac `n'`
-        \\ share_mem_store_compile_correct_tac `"MappedWrite"`
-            `t1 with pc := p + n2w (LENGTH bytes + pos_val s1.pc 0 code2)`
-            `dimindex (:α) DIV 8`
-            `s1.ffi with
-              <|ffi_state := ffi';
-                io_events :=
-                  s1.ffi.io_events ++
-                  [IO_event "MappedWrite"
-                    [n2w (dimindex (:α) DIV 8)]
-                    (ZIP (w2wlist_le (t1.regs n') (dimindex (:α) DIV 8) ++
-                          addr2w8list (c + t1.regs n''),v4))]|>` )
-      >- (rfs[good_dimindex_def] >> fs[])
-      >- enc_is_valid_mapped_access_tac
-      >- ( `t1.regs n' = w` by reg_val_tac `n'`
-        \\ gvs[apply_oracle_def,call_FFI_def,LENGTH_APPEND,good_dimindex_def]
-      )
-      >- (rfs[good_dimindex_def] >> fs[])
-      >- enc_is_valid_mapped_access_tac
-      >- ( `t1.regs n' = w` by reg_val_tac `n'`
-        \\ gvs[apply_oracle_def,call_FFI_def,LENGTH_APPEND,good_dimindex_def]
-      )
-    )
-    >- ( (* Store8 *)
-      gvs[pair_case_eq,option_case_eq, ffi_result_case_eq]
-      \\ share_mem_eval_expand_tac
-      \\ `t1.regs n'' = w'` by reg_val_tac `n''`
-      \\ simp[]
-      >- enc_is_valid_mapped_access_tac
-      >- (
-        `t1.regs n'' = w'` by reg_val_tac `n''`
-        \\ `t1.regs n' = w` by reg_val_tac `n'`
-        \\ share_mem_store_compile_correct_tac `"MappedWrite"`
-            `t1 with pc := p + n2w (LENGTH bytes + pos_val s1.pc 0 code2)`
-            `1`
-            `s1.ffi with
-              <|ffi_state := ffi';
-                io_events :=
-                  s1.ffi.io_events ++
-                  [IO_event "MappedWrite"
-                    [1w]
-                    (ZIP (w2wlist_le (t1.regs n') 1 ++
-                          addr2w8list (c + t1.regs n''),v4))]|>` )
-      >- enc_is_valid_mapped_access_tac
-      >- ( `t1.regs n' = w` by reg_val_tac `n'`
-        \\ gvs[apply_oracle_def,call_FFI_def,LENGTH_APPEND,good_dimindex_def]
-      )
-      >- enc_is_valid_mapped_access_tac
-      >- ( `t1.regs n' = w` by reg_val_tac `n'`
-        \\ gvs[apply_oracle_def,call_FFI_def,LENGTH_APPEND,good_dimindex_def]
-      )
-    )
-  )
+   (say "share_mem_op"
+    \\ Cases_on `m` >>
+    fs[share_mem_op_def,share_mem_load_def,share_mem_store_def]>>
+    gvs[pair_case_eq,option_case_eq, ffi_result_case_eq,CaseEq"word_loc"]>>
+     fs[asm_fetch_def,state_rel_def]>>
+     drule_all IMP_bytes_in_memory_ShareMem>>strip_tac>>
+     fs[share_mem_domain_code_rel_def]>>
+     qpat_assum `!pc op re a inst len i. asm_fetch_aux _ _ = SOME _ /\
+     mmio_pcs_min_index _ = SOME _ ==> _` drule_all>>strip_tac>>
+     fs[get_memop_info_def]>>
+     drule find_index_is_MEM>>strip_tac>>
+     simp[Once targetSemTheory.evaluate_def]>>
+     qpat_x_assum ‘target_state_rel _ _ _’ assume_tac>>
+     fs[target_state_rel_def]>>
+
+    qpat_assum ‘share_mem_state_rel _ _ _ _ ’ assume_tac>>
+    fs[share_mem_state_rel_def]>>
+    qpat_assum `!index' i'. mmio_pcs_min_index _ = SOME i' /\ index' < _ /\
+    _ ==> _` $ qspecl_then [`index`, `i`] drule>>
+
+   (impl_tac>-(drule find_index_LESS_LENGTH >> fs[]))>>
+    strip_tac>>
+    `mc_conf.target.get_pc ms1 <> mc_conf.ccache_pc /\
+    mc_conf.target.get_pc ms1 <> mc_conf.halt_pc` by (
+      irule ffi_entry_pcs_NOT_ccache_OR_halt_pc >> gvs[])>>
+    fs[]>>
+
+    Cases_on ‘a'’>>
+    fs[labSemTheory.addr_def,CaseEq"word_loc"]>>
+    qpat_assum ‘∀r. word_loc_val _ _ _ = SOME _’ $ qspec_then ‘n''’ assume_tac>>
+    TRY (qpat_assum ‘∀r. word_loc_val _ _ _ = SOME _’ $ qspec_then ‘n'’ assume_tac)>>
+    fs[option_case_eq,CaseEq"word_loc"]>>
+    qpat_x_assum ‘read_reg n'' _ = _ ’ $ assume_tac>>
+    TRY (qpat_x_assum ‘read_reg n' _ = _ ’ $ assume_tac)>>
+    fs[word_loc_val_def]>>
+    qpat_x_assum ‘_ = v'’ $ assume_tac o GSYM>>
+
+    qpat_assum ‘asm_ok _ _’ mp_tac>>
+    rewrite_tac[asm_ok_def,inst_ok_def,reg_ok_def]>>strip_tac>>
+    rfs[]>>
+    ‘∀x. word_to_bytes_aux 1n x F = [get_byte 0w x F]’
+      by (rewrite_tac[word_to_bytes_aux_def,ONE]>>simp[])>>
+    fs[]
+    >>~- ([‘Halt (FFI_outcome _)’],
+          IF_CASES_TAC>>fs[]>>
+          pop_assum irule>>
+          enc_is_valid_mapped_access_tac>>fs[])>>
+
+    simp[bool_case_eq]>>
+    simp[GSYM PULL_EXISTS]>>
+    (conj_asm1_tac >-
+      enc_is_valid_mapped_access_tac)>>fs[]>>
+    pairarg_tac>>fs[inc_pc_def,dec_clock_def]>>
+    irule_at Any EQ_SYM>>
+    simp[Once SWAP_EXISTS_THM]>>
+    last_x_assum $ irule>>fs[]>>
+    (conj_tac >-
+     (rpt strip_tac>>
+      first_x_assum $ irule o cj 1>>
+      first_assum $ irule_at Any>>
+      metis_tac[]))>>
+      rename1 ‘apply_oracle _ _ = (ms1', new_oracle)’>>
+    (conj_tac >-
+     (rpt gen_tac>>strip_tac>>
+      fs[apply_oracle_def,shift_seq_def]>>
+      qpat_x_assum ‘_ = new_oracle’ $ assume_tac o GSYM>>fs[]>>
+      first_x_assum irule>>
+      fs[]>>
+      irule (cj 2 RTC_RULES)>>
+      rfs[evaluatePropsTheory.call_FFI_rel_def]>>
+      last_assum $ irule_at Any>>fs[]))>>
+    (conj_tac >-
+     (rpt gen_tac>>strip_tac>>
+      fs[apply_oracle_def,shift_seq_def]>>
+      qpat_x_assum ‘_ = new_oracle’ $ assume_tac o GSYM>>fs[]>>
+      first_x_assum irule>>fs[]>>
+      first_x_assum $ irule_at Any>>
+      irule (cj 2 RTC_RULES)>>
+      rfs[evaluatePropsTheory.call_FFI_rel_def]>>
+      last_assum $ irule_at Any>>fs[]))>>
+
+    fs[apply_oracle_def,shift_seq_def]>>
+    qpat_x_assum ‘_ = ms1'’ $ assume_tac o GSYM>>fs[]>>
+    qpat_x_assum ‘∀a b c d e f g h i j k l. _ ⇒ _’ mp_tac>>
+    disch_then $ drule>>fs[]>>
+    drule find_index_LESS_LENGTH>>strip_tac>>
+    simp[target_state_rel_def]>>
+
+    strip_tac>>
+    (conj_tac >-
+     (pop_assum $ irule o cj 1>>
+      fs[find_index_INDEX_OF, INDEX_OF_eq_SOME]>>
+      rpt (last_x_assum $ irule_at Any)>>fs[]))>>
+
+    qabbrev_tac ‘pc = p + n2w (LENGTH bytes + pos_val s1.pc 0n code2)’>>
+    qmatch_asmsub_abbrev_tac ‘call_FFI _ _ [nb] _ = _’>>
+    last_x_assum $ qspecl_then [‘ms1’, ‘0’, ‘index’, ‘new_bytes’, ‘t1’, ‘nb’, ‘n''’, ‘c’, ‘n'’, ‘pc’, ‘s1.ffi’, ‘new_ffi’] mp_tac>>
+    (impl_tac>-
+      fs[target_state_rel_def,find_index_INDEX_OF, INDEX_OF_eq_SOME])>>
+    strip_tac>>rfs[Abbr ‘nb’]>>
+    qmatch_asmsub_abbrev_tac ‘target_state_rel mc_conf.target t1_new’>>
+    qexistsl [‘code2’, ‘labs’, ‘t1_new’] >> fs[]>>
+    fs[Abbr ‘t1_new’]>>
+    qpat_x_assum ‘∀a b c d e f. _ ⇒ _’ mp_tac>>
+    ‘call_FFI_rel꙳ s1.ffi s1.ffi’ by fs[cj 1 RTC_RULES]>>
+    rpt (disch_then $ drule_at Any)>>
+    fs[find_index_INDEX_OF, INDEX_OF_eq_SOME]>>
+    fs[target_state_rel_def,UPDATE_def]>>
+    rw[word_loc_val_def]>>
+    metis_tac[word_loc_val_def])
   THEN1 (* Jump *)
    (say "Jump"
     \\ qmatch_assum_rename_tac
@@ -8312,7 +8105,7 @@ QED
 Definition line_to_info_def:
   line_to_info (secs: 'a sec list) p x = case SND x of
     SOME (Asm (ShareMem m r ad) bytes l) =>
-      let (name,nb) = get_memop_info m (:'a) in
+      let (name,nb) = get_memop_info m in
       [(name,
        <|entry_pc := n2w (pos_val (FST x) p secs)
         ;nbytes:=nb
@@ -8398,7 +8191,7 @@ Proof
     gvs[pos_val_def,line_length_def] >>
     gvs[all_enc_ok_def,line_ok_def,line_length_def] >>
     gvs[get_shmem_info_def] >>
-    qpat_abbrev_tac `memop_info = get_memop_info m (:α)` >>
+    qpat_abbrev_tac `memop_info = get_memop_info m` >>
     Cases_on `memop_info` >>
     gvs[UNZIP_MAP] >>
     last_x_assum $ qspec_then `p' + LENGTH bytes` mp_tac >>
@@ -8457,7 +8250,7 @@ QED
 Theorem MEM_get_shmem_info:
   all_enc_ok c labs ffis p' (code2: 'a sec list) /\
   asm_fetch_aux pc code2 = SOME (Asm (ShareMem op re a) inst' len) /\
-  get_memop_info op (:'a) = (q,r:word8) ==>
+  get_memop_info op = (q,r:word8) ==>
   MEM
     (q,
     <|entry_pc:=n2w (pos_val pc p code2)
@@ -8618,7 +8411,7 @@ Theorem get_shmem_info_ok_lemma:
     (?index.
       find_index (n2w p + n2w (pos_val pc 0 code2)) (MAP (\rec. rec.entry_pc) new_shmem_info) 0 =
         SOME index /\
-      (let (name, nb) = get_memop_info op (:'a) in
+      (let (name, nb) = get_memop_info op in
         EL (index+i) new_ffi_names = name /\
         EL index new_shmem_info =
           <|entry_pc := (EL index new_shmem_info).entry_pc
@@ -8641,7 +8434,7 @@ Proof
   rpt strip_tac >>
   gvs[EL_APPEND_EQN,word_add_n2w]
   >- (
-    Cases_on `(get_memop_info:memop -> 'a itself -> string # word8) op (:'a)` >>
+    Cases_on `(get_memop_info:memop -> string # word8) op` >>
     drule_all MEM_get_shmem_info >>
     strip_tac >>
     first_x_assum $ qspec_then `p` assume_tac >>
@@ -8978,7 +8771,7 @@ val IMP_state_rel_make_init = Q.prove(
       `n2w (pos_val pc 0 code2) + (mc_conf.target.get_pc ms: 'a word)`,
       `0`] assume_tac find_index_APPEND
     \\ gvs[AllCaseEqs()]
-    \\ Cases_on `get_memop_info op (:'a)`
+    \\ Cases_on `get_memop_info op`
     >- (
       drule find_index_shift
       \\ fs[]
@@ -9528,7 +9321,7 @@ Proof
   qspecl_then [`q`,`c.pos`,`[]`,`[]`] assume_tac get_shmem_info_FST_SND_LENGTH_eq >>
   gvs[] >>
   qpat_x_assum `MAP _ _ = DROP _ _` $
-    assume_tac o Q.AP_TERM `LENGTH` >> 
+    assume_tac o Q.AP_TERM `LENGTH` >>
   gvs[LENGTH_MAP,LENGTH_DROP]
 QED
 
